intermediate2/Zeta.Intermediate.Blum.fst
@@ -2,6 +2,7 @@ module Zeta.Intermediate.Blum
 
 open Zeta.Intermediate.Store
 open Zeta.Intermediate.StateRel
+open FStar.Classical
 
 module SA = Zeta.SeqAux
 module GV = Zeta.GenericVerifier
@@ -19,6 +20,27 @@ let lemma_spec_rel_implies_same_add_elem (#vcfg:_)
   = lemma_spec_rel_implies_prefix_spec_rel il i
 
 #push-options "--z3rlimit_factor 3"
+
+let lemma_spec_rel_implies_is_blum_evict_identical (#vcfg:_)
+  (il: verifiable_log vcfg {spec_rel il})
+  (i: seq_index il)
+  : Lemma (ensures (let ilk = to_logk il in
+                    is_blum_evict il i = is_blum_evict ilk i))
+  = let _il = prefix il i in
+    let t = src il i in
+    let _vss:IV.vtls_t vcfg = thread_state_pre t il i in
+    let _sts = _vss.st in
+    let e = index il i in
+    //let s = GV.evict_slot e in
+
+    lemma_cur_thread_state_extend il i;
+
+    let ilk = to_logk il in
+    let _ilk = SA.prefix ilk i in
+    let _vsk: HV.vtls_t vcfg.app = thread_state_pre t ilk i in
+    let _stk = _vsk.st in
+    let ek = index ilk i in
+    ()
 
 let lemma_spec_rel_implies_same_evict_elem (#vcfg:_)
   (il: verifiable_log vcfg {spec_rel il})
@@ -51,32 +73,65 @@ let lemma_spec_rel_implies_same_evict_elem (#vcfg:_)
 
 #pop-options
 
-let lemma_spec_rel_implies_same_add_seq (#vcfg:_) (ep: epoch) (il: verifiable_log vcfg)
+#push-options "--fuel 0 --ifuel 1 --query_stats"
+
+let rec lemma_spec_rel_implies_same_add_seq (#vcfg:_) (ep: epoch) (il: verifiable_log vcfg)
   : Lemma (requires (spec_rel il))
           (ensures (let ilk = to_logk il in
                     add_seq ep il == add_seq ep ilk))
-  = admit()
+          (decreases (length il))
+  = let ilk = to_logk il in
+    if length il = 0 then (
+      add_seq_empty ep il;
+      add_seq_empty ep ilk
+    )
+    else (
+      let i = length il - 1 in
+      let il' = prefix il i in
+      let ilk' = to_logk il' in
+      lemma_spec_rel_implies_same_add_seq ep il';
+      add_seq_snoc ep il;
+      add_seq_snoc ep ilk
+    )
 
-let lemma_spec_rel_implies_same_evict_seq (#vcfg:_) (ep: epoch) (il: verifiable_log vcfg)
+#pop-options
+
+let rec lemma_spec_rel_implies_same_evict_seq (#vcfg:_) (ep: epoch) (il: verifiable_log vcfg)
   : Lemma (requires (spec_rel il))
           (ensures (let ilk = to_logk il in
                     evict_seq ep il == evict_seq ep ilk))
-  = admit()
+          (decreases (length il))
+  = let ilk = to_logk il in
+    let ess = evict_seq ep il in
+    let esk = evict_seq ep ilk in
+    if length il = 0 then (
+      evict_seq_empty ep il;
+      evict_seq_empty ep ilk
+    )
+    else (
+      let i = length il - 1 in
+      let il' = prefix il i in
+      let ess' = evict_seq ep il' in
+      let ilk' = to_logk il' in
+      let esk' = evict_seq ep ilk' in
+      lemma_spec_rel_implies_same_evict_seq ep il';
+      assert(ess' == esk');
+      evict_seq_snoc ep il;
+      evict_seq_snoc ep ilk;
+      if is_blum_evict il i then
+        lemma_spec_rel_implies_same_evict_elem il i
+      else
+        lemma_spec_rel_implies_is_blum_evict_identical il i
+    )
 
 let lemma_spec_rel_implies_same_add_set (#vcfg:_) (ep: epoch) (il: verifiable_log vcfg)
   : Lemma (requires (spec_rel il))
           (ensures (let ilk = to_logk il in
                     add_set ep il == add_set ep ilk))
-  = admit()
+  = ()
 
 let lemma_spec_rel_implies_same_evict_set (#vcfg:_) (ep: epoch) (il: verifiable_log vcfg)
   : Lemma (requires (spec_rel il))
           (ensures (let ilk = to_logk il in
                     evict_set ep il == evict_set ep ilk))
-  = admit()
-
-let lemma_vtls_rel_implies_ms_verifiable (#vcfg:_) (ep: epoch) (ils:verifiable_log vcfg)
-  : Lemma (requires (forall_vtls_rel ils))
-          (ensures (let ilk = to_logk ils in
-                    GG.aems_equal_upto ep (to_glog ils) ==> GG.aems_equal_upto ep (to_glog ilk)))
-  = admit()
+  = ()
